set up applied_implies_input, use it in RaftLinearizable, and prove interesting case

raft/AppliedImpliesInputInterface.v
@@ -10,6 +10,25 @@ Section AppliedImpliesInputInterface.
   Context {one_node_params : OneNodeParams orig_base_params}.
   Context {raft_params : RaftParams orig_base_params}.
 
+  Section inner.
+    Variables client id : nat.
+    Variable i : input.
+
+    Definition correct_entry (e : entry) : Prop :=
+      eClient e = client /\
+      eId e = id /\
+      eInput e = i.
+
+    Definition applied_implies_input_state (net : network) : Prop :=
+      exists e,
+        correct_entry e /\
+        ((exists h, In e (log (nwState net h))) \/
+         (exists p entries, In p (nwPackets net) /\
+                            mEntries (pBody p) = Some entries /\
+                            In e entries)).
+
+  End inner.
+
   Class applied_implies_input_interface : Prop :=
     {
       applied_implies_input :
@@ -17,7 +36,7 @@ Section AppliedImpliesInputInterface.
           step_f_star step_f_init (failed, net) tr ->
           eClient e = client ->
           eId e = id ->
-          In e (applied_entries (nwState net)) ->
+          applied_implies_input_state client id (eInput e) net ->
           in_input_trace client id (eInput e) tr
     }.
 End AppliedImpliesInputInterface.
