raft/proof/AppliedImpliesInputProof.v
@@ -7,7 +7,7 @@ Require Import Omega.
 Require Import Net.
 Require Import Util.
 Require Import VerdiTactics.
-Require Import TraceRelations.
+Require Import InverseTraceRelations.
 
 Require Import Raft.
 Require Import CommonTheorems.
@@ -26,18 +26,247 @@ Section AppliedImpliesInputProof.
 
   Context {oiai : output_implies_applied_interface}.
 
+  Lemma in_input_trace_or_app :
+    forall c id i tr1 tr2,
+      in_input_trace c id i tr1 \/ in_input_trace c id i tr2 ->
+      in_input_trace c id i (tr1 ++ tr2).
+  Proof.
+    unfold in_input_trace.
+    intuition; break_exists_exists; intuition.
+  Qed.
+
   Section inner.
     Variables client id : nat.
+    Variable i : input.
 
-    Lemma applied_implies_input :
-      forall failed net tr e,
-        step_f_star step_f_init (failed, net) tr ->
-        eClient e = client ->
-        eId e = id ->
-        In e (applied_entries (nwState net)) ->
-        in_input_trace client id (eInput e) tr.
-    Admitted.
+    Lemma applied_implies_input_update_split :
+      forall client id i net h d ps,
+        applied_implies_input_state client id i (mkNetwork ps (update (nwState net) h d)) ->
+        exists e,
+          correct_entry client id i e /\
+          (In e (log d) \/
+           (exists h, In e (log (nwState net h))) \/
+           (exists p es, In p ps /\ mEntries (pBody p) = Some es /\ In e es)).
+    Proof.
+      unfold applied_implies_input_state.
+      intros.
+      break_exists_exists.
+      intuition.
+      break_exists.
+      simpl in *.
+      destruct (name_eq_dec h x0); rewrite_update; eauto.
+    Qed.
+
+    Lemma aiis_intro_state :
+      forall client id i net e h,
+        In e (log (nwState net h)) ->
+        correct_entry client id i e ->
+        applied_implies_input_state client id i net.
+    Proof.
+      unfold applied_implies_input_state.
+      eauto 10.
+    Qed.
+
+    Lemma aiis_intro_packet :
+      forall client id i net e p es,
+        In p (nwPackets net) ->
+        correct_entry client id i e ->
+        mEntries (pBody p) = Some es ->
+        In e es ->
+        applied_implies_input_state client id i net.
+    Proof.
+      unfold applied_implies_input_state.
+      eauto 10.
+    Qed.
+
+    Lemma doGenericServer_log :
+      forall h st os st' ps,
+        doGenericServer h st = (os, st', ps) ->
+        log st' = log st.
+    Proof.
+      intros. unfold doGenericServer in *.
+      repeat break_match; find_inversion;
+      use_applyEntries_spec; simpl in *;
+      subst; auto.
+    Qed.
+
+    Theorem handleTimeout_log :
+      forall h st out st' ps,
+        handleTimeout h st = (out, st', ps) ->
+        log st' = log st.
+    Proof.
+      intros. unfold handleTimeout, tryToBecomeLeader in *.
+      break_match; find_inversion; subst; auto.
+    Qed.
+
+    Theorem handleClientRequest_no_messages :
+      forall h st client id c out st' ps p,
+        handleClientRequest h st client id c = (out, st', ps) ->
+        In p ps -> False.
+    Proof.
+      unfold handleClientRequest.
+      intros.
+      break_match; find_inversion; simpl in *; intuition.
+    Qed.
+
+    Theorem handleClientRequest_log :
+      forall h st client id c out st' ps,
+        handleClientRequest h st client id c = (out, st', ps) ->
+        (log st' = log st \/
+         exists e,
+           log st' = e :: log st /\
+           eIndex e = S (maxIndex (log st)) /\
+           eTerm e = currentTerm st /\
+           eClient e = client /\
+           eInput e = c /\
+           eId e = id).
+    Proof.
+      intros. unfold handleClientRequest in *.
+      break_match; find_inversion; subst; intuition.
+      simpl in *. eauto 10.
+    Qed.
+
+    Theorem handleTimeout_not_is_append_entries :
+      forall h st st' ms m,
+        handleTimeout h st = (st', ms) ->
+        In m ms -> ~ is_append_entries (snd m).
+    Proof.
+      intros. unfold handleTimeout, tryToBecomeLeader in *.
+      break_match; find_inversion; subst; simpl in *; eauto;
+      repeat (do_in_map; subst; simpl in *); intuition; break_exists; congruence.
+    Qed.
+
+    Lemma mEntries_some_is_applied_entries :
+      forall m es,
+        mEntries m = Some es ->
+        is_append_entries m.
+    Proof.
+      unfold mEntries.
+      intros.
+      break_match; try discriminate.
+      find_inversion.
+      eauto 10.
+    Qed.
+
+    Lemma doGenericServer_packets :
+      forall h st os st' ps p,
+        doGenericServer h st = (os, st', ps) ->
+        In p ps -> False.
+    Proof.
+      intros. unfold doGenericServer in *.
+      repeat break_match; find_inversion; subst; auto.
+    Qed.
+
+    Lemma doLeader_messages :
+      forall d h os d' ms m es e,
+        doLeader d h = (os, d', ms) ->
+        In m ms ->
+        mEntries (snd m) = Some es ->
+        In e es ->
+        In e (log d).
+    Proof.
+      unfold doLeader.
+      intros.
+      repeat break_match; repeat find_inversion; simpl in *; intuition.
+      do_in_map. subst. simpl in *. find_inversion.
+      eauto using findGtIndex_in.
+    Qed.
+
+    Lemma handleInputs_aais :
+      forall client id h inp i net os d' ms e o,
+        ~ applied_implies_input_state client id i net ->
+        handleInput h inp (nwState net h) = (os, d', ms) ->
+        correct_entry client id i e ->
+        In e (log d') ->
+        in_input_trace client id i [(h, inl inp); o].
+    Proof.
+      intros.
+      destruct inp; simpl in *.
+      - find_erewrite_lem handleTimeout_log.
+        exfalso. eauto using aiis_intro_state.
+      - find_eapply_lem_hyp handleClientRequest_log.
+        break_or_hyp.
+        + find_rewrite.
+          exfalso. eauto using aiis_intro_state.
+        + break_exists. break_and. subst.
+          find_rewrite. simpl in *.
+          break_or_hyp.
+          * subst. unfold in_input_trace. unfold correct_entry in *.
+            break_and. subst. simpl. eauto.
+          * exfalso. eauto using aiis_intro_state.
+    Qed.
+
+    Lemma applied_implies_input_in_input_trace :
+      forall net failed net' failed' tr,
+        raft_intermediate_reachable net ->
+        @step_f _ _ failure_params (failed, net) (failed', net') tr ->
+        ~ applied_implies_input_state client id i net ->
+        applied_implies_input_state client id i net' ->
+        in_input_trace client id i tr.
+    Proof.
+      intros.
+      match goal with
+        | [ H : context [step_f _ _ _ ] |- _ ] => invcs H
+      end.
+      - admit.
+      - unfold RaftInputHandler in *. repeat break_let. subst. find_inversion.
+        find_apply_lem_hyp applied_implies_input_update_split.
+        break_exists. intuition; break_exists.
+        + find_erewrite_lem doLeader_same_log.
+          find_erewrite_lem doGenericServer_log.
+          eauto using handleInputs_aais.
+        + exfalso. eauto using aiis_intro_state.
+        + intuition. do_in_app. intuition.
+          * do_in_map. subst. simpl in *.
+            { repeat (do_in_app; intuition).
+              - destruct inp; simpl in *.
+                + exfalso. eapply handleTimeout_not_is_append_entries; eauto.
+                  eauto using mEntries_some_is_applied_entries.
+                + exfalso. eauto using handleClientRequest_no_messages.
+              - exfalso. eauto using doGenericServer_packets.
+              - find_eapply_lem_hyp doLeader_messages; eauto.
+                find_erewrite_lem doGenericServer_log.
+                eauto using handleInputs_aais.
+            }
+          * exfalso. eauto using aiis_intro_packet.
+      - admit.
+      - admit.
+      - congruence.
+      - admit.
+    Qed.
+
+    Instance ITR : InverseTraceRelation step_f :=
+      { init := step_f_init;
+        R := fun s => applied_implies_input_state client id i (snd s);
+        T := in_input_trace client id i
+      }.
+    - intros. admit.  (* decidable R *)
+    - intros.
+      unfold in_input_trace in *. break_exists_exists.
+      intuition.
+    - unfold applied_implies_input_state. intro. break_exists. break_and.
+      intuition; break_exists; intuition.
+    - intros. simpl in *.
+      apply in_input_trace_or_app. right.
+      destruct s, s'. simpl in *.
+      eapply applied_implies_input_in_input_trace; eauto.
+      eapply step_f_star_raft_intermediate_reachable; eauto.
+    Defined.
   End inner.
+
+  Lemma applied_implies_input :
+    forall client id failed net tr e,
+      @step_f_star _ _ failure_params step_f_init (failed, net) tr ->
+      eClient e = client ->
+      eId e = id ->
+      applied_implies_input_state client id (eInput e) net ->
+      in_input_trace client id (eInput e) tr.
+  Proof.
+    intros.
+    pose proof @inverse_trace_relations_work _ _ step_f (ITR client id (eInput e)) (failed, net) tr.
+    unfold step_f_star in *. simpl in *.
+    auto.
+  Qed.
 
   Instance aiii : applied_implies_input_interface.
   Proof.
